chore: Address PR feedback from #1427

AwsCryptographicMaterialProviders/dafny/AwsCryptographyKeyStoreAdmin/src/CreateKeysHV2.dfy
@@ -4,6 +4,8 @@
 include "../Model/AwsCryptographyKeyStoreAdminTypes.dfy"
 include "../../AwsCryptographyKeyStore/Model/AwsCryptographyKeyStoreTypes.dfy"
 include "../../../../AwsCryptographyPrimitives/Model/AwsCryptographyPrimitivesTypes.dfy"
+include "BKSAOperationUtils.dfy"
+include "KmsUtils.dfy"
 
 module {:options "/functionSyntax:4" } CreateKeysHV2 {
   // Standard Library Imports
@@ -30,23 +32,26 @@ module {:options "/functionSyntax:4" } CreateKeysHV2 {
     // (Branch) Key Store Admin Imports
   import HvUtils = HierarchicalVersionUtils
   import Types = AwsCryptographyKeyStoreAdminTypes
+  import OptUtils = BKSAOperationUtils
+  import KmsUtils
 
-  datatype CryptoAndKMS = CryptoAndKMS(
+  /** Constrains the relationship of the Crypto & KMS client, 
+    ensuring they a valid but their histories are separate.
+    Also allows us to make claims about the Grant Tokens and kmsConfig. */
+  datatype CryptoAndKms = CryptoAndKms(
     kmsConfig: KeyStoreTypes.KMSConfiguration,
-    grantTokens: KMS.Types.GrantTokenList,
-    kms: KMS.Types.IKMSClient,
-    Crypto: AtomicPrimitives.AtomicPrimitivesClient
+    kms: KmsUtils.keyManagerStrat,
+    crypto: AtomicPrimitives.AtomicPrimitivesClient
   ) {
     ghost predicate ValidState()
     {
       && kms.ValidState()
-      && KMS.Types.IsValid_GrantTokenList(grantTokens)
       && KMSKeystoreOperations.HasKeyId(kmsConfig)
       && KmsArn.ValidKmsArn?(KMSKeystoreOperations.GetKeyId(kmsConfig))
-      && kms.Modifies !! Crypto.Modifies
-      && Crypto.ValidState()
+      && kms.Modifies !! crypto.Modifies
+      && crypto.ValidState()
     }
-    ghost const Modifies := multiset(kms.Modifies) + multiset(Crypto.Modifies)
+    ghost const Modifies := multiset(kms.Modifies) + multiset(crypto.Modifies)
   }
 
   function ConvertKmsErrorToError(
@@ -72,36 +77,28 @@ module {:options "/functionSyntax:4" } CreateKeysHV2 {
 
   // TODO-HV-2-GA: Update Specification for HV-2 Branch Key Creation
   method CreateBranchAndBeaconKeys(
-    branchKeyIdentifier: string,
-    encryptionContext: map<string, string>,
-    timestamp: string,
-    branchKeyVersion: string,
-    logicalKeyStoreName: string,
-    kmsConfiguration: KeyStoreTypes.KMSConfiguration,
-    grantTokens: KMS.Types.GrantTokenList,
-    kmsClient: KMS.Types.IKMSClient,
-    storage: KeyStoreTypes.IKeyStorageInterface,
-    hierarchyVersion: KeyStoreTypes.HierarchyVersion
+    nameonly branchKeyIdentifier: string,
+    nameonly encryptionContext: map<string, string>,
+    nameonly timestamp: string,
+    nameonly branchKeyVersion: string,
+    nameonly logicalKeyStoreName: string,
+    nameonly kmsConfiguration: KeyStoreTypes.KMSConfiguration,
+    nameonly keyManagerAndStorage: OptUtils.KeyManagerAndStorage,
+    nameonly hierarchyVersion: KeyStoreTypes.HierarchyVersion
   )
     returns (output: Result<Types.CreateKeyOutput, Types.Error>)
-    // Generic Stateful pre and post conditions
     requires
-      && kmsClient.ValidState()
-      && storage.ValidState()
-      && kmsClient.Modifies !! storage.Modifies
-    modifies multiset(storage.Modifies) + multiset(kmsClient.Modifies)
-    ensures
-      && storage.ValidState()
-      && kmsClient.ValidState()
-      && kmsClient.Modifies !! storage.Modifies
-    // 
-    requires
+      // TODO-HV-2-M? : Support KmsDecryptEncrypt?
+      && keyManagerAndStorage.keyManagerStrat.kmsSimple?
+      && keyManagerAndStorage.ValidState()
       && KMSKeystoreOperations.HasKeyId(kmsConfiguration)
       && KmsArn.ValidKmsArn?(KMSKeystoreOperations.GetKeyId(kmsConfiguration))
       && hierarchyVersion.v2?
       && 0 < |branchKeyIdentifier|
       && 0 < |branchKeyVersion|
       && forall k <- encryptionContext :: DDB.Types.IsValid_AttributeName(Structure.ENCRYPTION_CONTEXT_PREFIX + k)
+    modifies keyManagerAndStorage.Modifies
+    ensures keyManagerAndStorage.ValidState()
   {
     // Construct Branch Key Contexts for ACTIVE, Version and Beacon items.
     var decryptOnlyBranchKeyContext := Structure.DecryptOnlyBranchKeyEncryptionContext(
@@ -141,30 +138,30 @@ module {:options "/functionSyntax:4" } CreateKeysHV2 {
       e => Types.AwsCryptographyPrimitives(
           AwsCryptographyPrimitives := e));
 
-    var CryptoAndKMS := CryptoAndKMS(kmsConfiguration, grantTokens, kmsClient, crypto);
+    var CryptoAndKms := CryptoAndKms(kmsConfiguration, keyManagerAndStorage.keyManagerStrat, crypto);
     var decrytOnlyBKItem :- packAndCallKMS(
       branchKeyContext := decryptOnlyBranchKeyContext,
-      CryptoAndKMS := CryptoAndKMS,
+      cryptoAndKms := CryptoAndKms,
       material := activePlaintextMaterial,
       encryptionContext := encryptionContext
     );
 
     var activeBKItem :- packAndCallKMS(
       branchKeyContext := activeBranchKeyContext,
-      CryptoAndKMS := CryptoAndKMS,
+      cryptoAndKms := CryptoAndKms,
       material := activePlaintextMaterial,
       encryptionContext := encryptionContext
     );
 
     var beaconBKItem :- packAndCallKMS(
       branchKeyContext := beaconBranchKeyContext,
-      CryptoAndKMS := CryptoAndKMS,
+      cryptoAndKms := CryptoAndKms,
       material := beaconPlaintextMaterial,
       encryptionContext := encryptionContext
     );
 
     // Write ACTIVE, Version & Beacon Items to storage
-    var writeItems? := storage.WriteNewEncryptedBranchKey(
+    var writeItems? := keyManagerAndStorage.storage.WriteNewEncryptedBranchKey(
       KeyStoreTypes.WriteNewEncryptedBranchKeyInput(
         Active := activeBKItem,
         Version := decrytOnlyBKItem,
@@ -175,9 +172,10 @@ module {:options "/functionSyntax:4" } CreateKeysHV2 {
       e => Types.AwsCryptographyKeyStore(
           AwsCryptographyKeyStore:= e
         ));
-
+    // By making this ghost, we avoid the Dafny transpiler emitting in Java etc.
+    ghost var storage := keyManagerAndStorage.storage;
     assert |storage.History.WriteNewEncryptedBranchKey| == |old(storage.History.WriteNewEncryptedBranchKey)| + 1;
-    ghost var writeEvent := storage.History.WriteNewEncryptedBranchKey[-1 % |storage.History.WriteNewEncryptedBranchKey|];
+    ghost var writeEvent := Seq.Last(storage.History.WriteNewEncryptedBranchKey);
     assert
       && writeEvent.output.Success?
       && writeEvent.input.Active == activeBKItem
@@ -192,42 +190,44 @@ module {:options "/functionSyntax:4" } CreateKeysHV2 {
 
   method packAndCallKMS(
     nameonly branchKeyContext: map<string, string>,
-    nameonly CryptoAndKMS: CryptoAndKMS,
+    nameonly cryptoAndKms: CryptoAndKms,
     nameonly material: seq<uint8>,
     nameonly encryptionContext: map<string, string>
   )
     returns (output: Result<KeyStoreTypes.EncryptedHierarchicalKey, Types.Error>)
-
-    requires CryptoAndKMS.ValidState()
-    modifies CryptoAndKMS.Modifies
-    ensures CryptoAndKMS.ValidState()
-
     requires
+      && cryptoAndKms.ValidState()
       && Structure.BranchKeyContext?(branchKeyContext)
       && |material| == Structure.AES_256_LENGTH as int
-      && KMSKeystoreOperations.AttemptKmsOperation?(CryptoAndKMS.kmsConfig, branchKeyContext[Structure.KMS_FIELD])
-      && KMSKeystoreOperations.GetKeyId(CryptoAndKMS.kmsConfig) == branchKeyContext[Structure.KMS_FIELD]
-
-    // TODO-HV-2-GA: Update Specification for HV-2 Branch Key Creation
-    ensures output.Success? ==>
-              && |CryptoAndKMS.kms.History.Encrypt| == |old(CryptoAndKMS.kms.History.Encrypt)| + 1
-              && var kmsEvent :=  CryptoAndKMS.kms.History.Encrypt[-1 % |CryptoAndKMS.kms.History.Encrypt|];
-              && kmsEvent.output.Success?
-              && var kmsInput := kmsEvent.input;
-              && KMSKeystoreOperations.Compatible?(CryptoAndKMS.kmsConfig, kmsInput.KeyId)
-              && |kmsInput.Plaintext| == (Structure.BKC_DIGEST_LENGTH + Structure.AES_256_LENGTH) as int
-              && kmsInput.EncryptionContext == Some(encryptionContext)
-              && kmsInput.GrantTokens == Some(CryptoAndKMS.grantTokens)
-              && kmsEvent.output.value.CiphertextBlob.Some?
-              && var digest := kmsInput.Plaintext[..Structure.BKC_DIGEST_LENGTH];
-              && material == kmsInput.Plaintext[Structure.BKC_DIGEST_LENGTH..]
-              && |CryptoAndKMS.Crypto.History.Digest| == |old(CryptoAndKMS.Crypto.History.Digest)| + 1
-              && var digestEvent := CryptoAndKMS.Crypto.History.Digest[-1 % |CryptoAndKMS.Crypto.History.Digest|];
-              && digestEvent.output.Success?
-              && digestEvent.output.value == digest
-              && digestEvent.input.digestAlgorithm == AtomicPrimitives.Types.SHA_384
+      && KMSKeystoreOperations.AttemptKmsOperation?(cryptoAndKms.kmsConfig, branchKeyContext[Structure.KMS_FIELD])
+      && KMSKeystoreOperations.GetKeyId(cryptoAndKms.kmsConfig) == branchKeyContext[Structure.KMS_FIELD]
+         // TODO-HV-2-M? : Support KmsDecryptEncrypt?
+      && cryptoAndKms.kms.kmsSimple?
+    modifies cryptoAndKms.Modifies
+    // Note: even if the method fails, the clients are ValidState
+    ensures cryptoAndKms.ValidState()
+    ensures
+         // TODO-HV-2-GA: Update Specification for HV-2 Branch Key Creation
+      && output.Success? ==>
+        && var kms := cryptoAndKms.kms.kmsSimple.kmsClient;
+        && |kms.History.Encrypt| == |old(kms.History.Encrypt)| + 1
+        && var kmsEvent :=  Seq.Last(kms.History.Encrypt);
+        && kmsEvent.output.Success?
+        && var kmsInput := kmsEvent.input;
+        && KMSKeystoreOperations.Compatible?(cryptoAndKms.kmsConfig, kmsInput.KeyId)
+        && |kmsInput.Plaintext| == (Structure.BKC_DIGEST_LENGTH + Structure.AES_256_LENGTH) as int
+        && kmsInput.EncryptionContext == Some(encryptionContext)
+        && kmsInput.GrantTokens == Some(cryptoAndKms.kms.kmsSimple.grantTokens)
+        && kmsEvent.output.value.CiphertextBlob.Some?
+        && var digest := kmsInput.Plaintext[..Structure.BKC_DIGEST_LENGTH];
+        && material == kmsInput.Plaintext[Structure.BKC_DIGEST_LENGTH..]
+        && |cryptoAndKms.crypto.History.Digest| == |old(cryptoAndKms.crypto.History.Digest)| + 1
+        && var digestEvent := Seq.Last(cryptoAndKms.crypto.History.Digest);
+        && digestEvent.output.Success?
+        && digestEvent.output.value == digest
+        && digestEvent.input.digestAlgorithm == AtomicPrimitives.Types.SHA_384
   {
-    var digest? := HvUtils.CreateBKCDigest(branchKeyContext, CryptoAndKMS.Crypto);
+    var digest? := HvUtils.CreateBKCDigest(branchKeyContext, cryptoAndKms.crypto);
     var digest :- digest?.MapFailure(
       e => Types.AwsCryptographyKeyStore(
           AwsCryptographyKeyStore:= e));
@@ -236,9 +236,9 @@ module {:options "/functionSyntax:4" } CreateKeysHV2 {
       plaintextTuple,
       encryptionContext,
       branchKeyContext[Structure.KMS_FIELD],
-      CryptoAndKMS.kmsConfig,
-      CryptoAndKMS.grantTokens,
-      CryptoAndKMS.kms
+      cryptoAndKms.kmsConfig,
+      cryptoAndKms.kms.kmsSimple.grantTokens,
+      cryptoAndKms.kms.kmsSimple.kmsClient
     );
     var wrappedMaterial :- wrappedMaterial?.MapFailure(e => ConvertKmsErrorToError(e));
     return Success(Structure.ConstructEncryptedHierarchicalKey(branchKeyContext, wrappedMaterial));
